<?xml version="1.0"?>
<rdf:RDF xmlns="https://kgrid.org/koio#"
     xml:base="https://kgrid.org/koio"
     xmlns:dc="http://purl.org/dc/elements/1.1/"
     xmlns:efo="http://www.ebi.ac.uk/efo/"
     xmlns:obo="http://purl.obolibrary.org/obo/"
     xmlns:owl="http://www.w3.org/2002/07/owl#"
     xmlns:rdf="http://www.w3.org/1999/02/22-rdf-syntax-ns#"
     xmlns:swo="http://www.ebi.ac.uk/swo/"
     xmlns:xml="http://www.w3.org/XML/1998/namespace"
     xmlns:xsd="http://www.w3.org/2001/XMLSchema#"
     xmlns:foaf="http://xmlns.com/foaf/0.1/"
     xmlns:rdfs="http://www.w3.org/2000/01/rdf-schema#"
     xmlns:skos="http://www.w3.org/2004/02/skos/core#"
     xmlns:swrla="http://swrl.stanford.edu/ontologies/3.3/swrla.owl#"
     xmlns:dcterms="http://purl.org/dc/terms/"
     xmlns:protege="http://protege.stanford.edu/plugins/owl/protege#"
     xmlns:subsets="http://purl.obolibrary.org/obo/ro/subsets#"
     xmlns:oboInOwl="http://www.geneontology.org/formats/oboInOwl#"
     xmlns:edamontology="http://edamontology.org#">
    <owl:Ontology rdf:about="https://kgrid.org/koio">
        <owl:versionIRI rdf:resource="http://www.kgrid.org/koio/2.1/koio.owl"/>
        <owl:imports rdf:resource="http://purl.obolibrary.org/obo/iao/2022-11-07/iao.owl"/>
        <owl:imports rdf:resource="https://raw.githubusercontent.com/allysonlister/swo/master/swo-full.owl"/>
        <dcterms:contributor>Allen Flynn</dcterms:contributor>
        <dcterms:contributor>Charles P. Friedman</dcterms:contributor>
        <dcterms:contributor>Farid Seifi</dcterms:contributor>
        <dcterms:contributor>Marisa Conte</dcterms:contributor>
        <dcterms:contributor>Peter Boisvert</dcterms:contributor>
        <dcterms:publisher>Knowledge Systems Lab. Department of Learning Health Sciences. University of Michigan Medical School.
https://knowledge-systems.lab.medicine.umich.edu/</dcterms:publisher>
        <dcterms:title>Knowledge Object Implementation Ontology (KOIO)</dcterms:title>
        <rdfs:comment>KOIO is a domain ontology that tells us what a Knowledge Object is as an artifact. It describes Knowledge Objects and their parts as they are implemented. For this reason, KOIO generally serves as an evolving formal and explicit model of Knowledge Objects. It can be used to describe the parts of many computable biomedical knowledge (CBK) artifacts found in the wild. In addition, KOIO functions as a formal specification for linked metadata relevant for describing, annotating, packaging, and handling CBK artifacts.

The Knowledge Systems Lab (KSL) at the University of Michigan began work on KOIO in 2016 and continues to evolve KOIO over time. KSL’s general approach is to keep KOIO concise, connected, and common.

To keep it concise, only a very small number of new terms describing key parts known to be valuable to CBK stakeholders are included in KOIO. These KOIO-defined terms include “Knowledge”, “Service”, and “Test”. As a model of Knowledge Objects, KOIO supports multiplicity of these parts meaning that a Knowledge Object may have one or more elements of knowledge plus multiple corresponding services and tests. KOIO enables the lifecycles and provenance of the key individual parts of Knowledge Objects to be tracked and documented independently.

The key parts of Knowledge Objects defined in KOIO are logically connected to terms from the upper-level Basic Formal Ontology (BFO). In addition, KOIO adopts terms from the Information Artifact Ontology (IAO) and the Software Ontology (SWO) wherever possible.

Finally, KOIO tries to leave implementation details out so that it can serve as a common ontology for describing nearly all CBK artifacts, regardless of the platforms or applications that support and incorporate them.</rdfs:comment>
        <owl:versionInfo rdf:datatype="http://www.w3.org/2001/XMLSchema#decimal">2.1</owl:versionInfo>
    </owl:Ontology>
    


    <!-- 
    ///////////////////////////////////////////////////////////////////////////////////////
    //
    // Annotation properties
    //
    ///////////////////////////////////////////////////////////////////////////////////////
     -->

    


    <!-- http://purl.org/dc/terms/publisher -->

    <owl:AnnotationProperty rdf:about="http://purl.org/dc/terms/publisher"/>
    


    <!-- http://www.w3.org/2000/01/rdf-schema#type -->

    <owl:AnnotationProperty rdf:about="http://www.w3.org/2000/01/rdf-schema#type"/>
    


    <!-- 
    ///////////////////////////////////////////////////////////////////////////////////////
    //
    // Object Properties
    //
    ///////////////////////////////////////////////////////////////////////////////////////
     -->

    


    <!-- http://purl.obolibrary.org/obo/RO_0002502 -->

    <rdf:Description rdf:about="http://purl.obolibrary.org/obo/RO_0002502">
        <rdfs:domain rdf:resource="https://kgrid.org/koio#Service"/>
        <rdfs:range rdf:resource="https://kgrid.org/koio#Knowledge"/>
        <obo:IAO_0000115>depends on, def., indicates that a service uses a specific knowledge</obo:IAO_0000115>
    </rdf:Description>
    


    <!-- http://www.ebi.ac.uk/swo/SWO_0000085 -->

    <rdf:Description rdf:about="http://www.ebi.ac.uk/swo/SWO_0000085">
        <rdfs:domain rdf:resource="https://kgrid.org/koio#Knowledge"/>
        <rdfs:domain rdf:resource="https://kgrid.org/koio#Service"/>
        <rdfs:domain rdf:resource="https://kgrid.org/koio#Test"/>
        <rdfs:range rdf:resource="https://kgrid.org/koio#Implementation"/>
        <obo:IAO_0000115>Note: KSL added this definition to contextualize the definition below from SWO.
implemented by, def., is the relationship between an abstract KO component and a piece of software (or computer processable content)  which includes an implementation of that abstract KO component for use when processed by a computer.</obo:IAO_0000115>
    </rdf:Description>
    


    <!-- http://www.ebi.ac.uk/swo/SWO_0004001 -->

    <rdf:Description rdf:about="http://www.ebi.ac.uk/swo/SWO_0004001">
        <rdfs:domain rdf:resource="https://kgrid.org/koio#Service"/>
        <rdfs:range rdf:resource="http://www.ebi.ac.uk/swo/SWO_9000050"/>
    </rdf:Description>
    


    <!-- https://kgrid.org/koio#hasDocumentation -->

    <owl:ObjectProperty rdf:about="https://kgrid.org/koio#hasDocumentation">
        <rdfs:subPropertyOf rdf:resource="http://purl.obolibrary.org/obo/BFO_0000051"/>
        <rdfs:domain rdf:resource="https://kgrid.org/koio#Implementation"/>
        <rdfs:domain rdf:resource="https://kgrid.org/koio#Knowledge"/>
        <rdfs:domain rdf:resource="https://kgrid.org/koio#KnowledgeObject"/>
        <rdfs:domain rdf:resource="https://kgrid.org/koio#Service"/>
        <rdfs:domain rdf:resource="https://kgrid.org/koio#Test"/>
        <rdfs:range rdf:resource="https://kgrid.org/koio#InformationArtifact"/>
        <obo:IAO_0000115>hasDocumentation, def., a property that indicates an association between a knowledge object, knowledge, or service and documentation that describes, relates to, or provides information about each of these things.</obo:IAO_0000115>
        <rdfs:label>has documentation</rdfs:label>
        <rdfs:seeAlso>from SPDX find term hasDocumentation: https://spdx.github.io/spdx-spec/v3.0.1/model/Core/Vocabularies/RelationshipType/
from SPDX find term Documentation:
http://spdx.org/rdf/terms#documentation</rdfs:seeAlso>
    </owl:ObjectProperty>
    


    <!-- https://kgrid.org/koio#hasKnowledge -->

    <owl:ObjectProperty rdf:about="https://kgrid.org/koio#hasKnowledge">
        <rdfs:subPropertyOf rdf:resource="http://purl.obolibrary.org/obo/BFO_0000051"/>
        <rdfs:domain rdf:resource="https://kgrid.org/koio#KnowledgeObject"/>
        <rdfs:range rdf:resource="https://kgrid.org/koio#Knowledge"/>
        <obo:IAO_0000115>hasKnowledge, def., indicates that a Knowledge Object contains or is associated with specific Knowledge.</obo:IAO_0000115>
        <rdfs:label>has knowledge</rdfs:label>
    </owl:ObjectProperty>
    


    <!-- https://kgrid.org/koio#hasService -->

    <owl:ObjectProperty rdf:about="https://kgrid.org/koio#hasService">
        <rdfs:subPropertyOf rdf:resource="http://purl.obolibrary.org/obo/BFO_0000051"/>
        <rdfs:domain rdf:resource="https://kgrid.org/koio#KnowledgeObject"/>
        <rdfs:range rdf:resource="https://kgrid.org/koio#Service"/>
        <obo:IAO_0000115>hasService , def., a relation that holds between a whole KnowledgeObject and its Service part(s). Denotes that a KnowledgeObject includes or provides a specific Service.</obo:IAO_0000115>
        <rdfs:label>has service</rdfs:label>
    </owl:ObjectProperty>
    


    <!-- https://kgrid.org/koio#hasTest -->

    <owl:ObjectProperty rdf:about="https://kgrid.org/koio#hasTest">
        <rdfs:subPropertyOf rdf:resource="http://purl.obolibrary.org/obo/BFO_0000051"/>
        <rdfs:domain rdf:resource="https://kgrid.org/koio#Knowledge"/>
        <rdfs:domain rdf:resource="https://kgrid.org/koio#KnowledgeObject"/>
        <rdfs:domain rdf:resource="https://kgrid.org/koio#Service"/>
        <rdfs:range rdf:resource="https://kgrid.org/koio#Test"/>
        <obo:IAO_0000115>hasTest, def., a property that links a knowledge object, service, or knowledge to a specific test designed to evaluate its functionality, performance, or reliability. This property signifies that the component has an associated test to verify or validate its behavior.</obo:IAO_0000115>
        <rdfs:label>has test</rdfs:label>
        <rdfs:seeAlso>from SPDX find term hasTest:
https://spdx.github.io/spdx-spec/v3.0.1/model/Core/Vocabularies/RelationshipType/</rdfs:seeAlso>
    </owl:ObjectProperty>
    


    <!-- 
    ///////////////////////////////////////////////////////////////////////////////////////
    //
    // Data properties
    //
    ///////////////////////////////////////////////////////////////////////////////////////
     -->

    


    <!-- https://kgrid.org/koio#KOIOVersion -->

    <owl:DatatypeProperty rdf:about="https://kgrid.org/koio#KOIOVersion">
        <rdfs:subPropertyOf rdf:resource="http://www.w3.org/2002/07/owl#topDataProperty"/>
        <obo:IAO_0000115>The version of KOIO from which metadata is derived</obo:IAO_0000115>
        <rdfs:label>KOIO version</rdfs:label>
    </owl:DatatypeProperty>
    


    <!-- 
    ///////////////////////////////////////////////////////////////////////////////////////
    //
    // Classes
    //
    ///////////////////////////////////////////////////////////////////////////////////////
     -->

    


    <!-- https://kgrid.org/koio#Artifact -->

    <owl:Class rdf:about="https://kgrid.org/koio#Artifact">
        <rdfs:subClassOf rdf:resource="http://purl.obolibrary.org/obo/BFO_0000040"/>
        <obo:IAO_0000115>Artifact =def. a MaterialEntity created or modified or selected by some agent to realize a certain FUNCTION or ROLE (Examples: a key, a lock, a digital file stored on a particular computing machine, a screwdriver)


Smith &amp; Ceusters, Aboutness: Towards Foundations for the Information Artifact Ontology</obo:IAO_0000115>
        <rdfs:isDefinedBy rdf:resource="http://purl.obolibrary.org/obo/iao.owl"/>
        <rdfs:label xml:lang="en">artifact</rdfs:label>
    </owl:Class>
    


    <!-- https://kgrid.org/koio#Collection -->

    <owl:Class rdf:about="https://kgrid.org/koio#Collection">
        <rdfs:subClassOf rdf:resource="https://kgrid.org/koio#InformationArtifact"/>
        <obo:IAO_0000115>Collection = def. an InformationArtifact comprised of two or more InformationArtifacts and at least one collectionIdentifier</obo:IAO_0000115>
        <rdfs:isDefinedBy rdf:resource="http://kgrid.org/koio/1.0.0/"/>
        <rdfs:label xml:lang="en">collection</rdfs:label>
    </owl:Class>
    


    <!-- https://kgrid.org/koio#Implementation -->

    <owl:Class rdf:about="https://kgrid.org/koio#Implementation">
        <rdfs:subClassOf rdf:resource="https://kgrid.org/koio#InformationArtifact"/>
        <owl:disjointWith rdf:resource="https://kgrid.org/koio#KnowledgeObject"/>
        <obo:IAO_0000115>def., a computer or machine processable file that is or informs a series of instructions that can be directly interpreted or executed.</obo:IAO_0000115>
        <rdfs:isDefinedBy rdf:resource="http://kgrid.org/koio/1.0.0/"/>
        <rdfs:label>implementation</rdfs:label>
    </owl:Class>
    


    <!-- https://kgrid.org/koio#InformationArtifact -->

    <owl:Class rdf:about="https://kgrid.org/koio#InformationArtifact">
        <rdfs:subClassOf rdf:resource="https://kgrid.org/koio#Artifact"/>
        <obo:IAO_0000115>An InformationArtifact = def., an Artifact that is the IndependentContinuant bearer created as the result of one or more intentional processes. Examples: uniprot, the english language, the contents of this document or a printout of it, the temperature measurements from a weather balloon. For more information, see the project home page at https://github.com/information-artifact-ontology/IAO</obo:IAO_0000115>
        <rdfs:comment>Per KOIO, Knowledge Objects are InformationArtifacts by definition.</rdfs:comment>
        <rdfs:isDefinedBy rdf:resource="http://purl.obolibrary.org/obo/iao.owl"/>
        <rdfs:label xml:lang="en">information artifact</rdfs:label>
    </owl:Class>
    


    <!-- https://kgrid.org/koio#Knowledge -->

    <owl:Class rdf:about="https://kgrid.org/koio#Knowledge">
        <rdfs:subClassOf rdf:resource="http://purl.obolibrary.org/obo/IAO_0000030"/>
        <obo:IAO_0000115>Knowledge, def., information or understanding about a subject, obtained through experience or study.</obo:IAO_0000115>
        <rdfs:label>knowledge</rdfs:label>
    </owl:Class>
    


    <!-- https://kgrid.org/koio#KnowledgeObject -->

    <owl:Class rdf:about="https://kgrid.org/koio#KnowledgeObject">
        <rdfs:subClassOf rdf:resource="https://kgrid.org/koio#InformationArtifact"/>
        <rdfs:subClassOf>
            <owl:Restriction>
                <owl:onProperty rdf:resource="https://kgrid.org/koio#hasKnowledge"/>
                <owl:someValuesFrom rdf:resource="https://kgrid.org/koio#Knowledge"/>
            </owl:Restriction>
        </rdfs:subClassOf>
        <obo:IAO_0000115>KnowledgeObject = def., an Information Artifact capable of serving a role as the atomic unit of computable knowledge and therefore comprised of at least one KnowledgeObjectImplementation</obo:IAO_0000115>
        <rdfs:isDefinedBy rdf:resource="http://kgrid.org/koio/1.0.0/"/>
        <rdfs:label xml:lang="en">knowledge object</rdfs:label>
    </owl:Class>
    


    <!-- https://kgrid.org/koio#KnowledgeObjectCollection -->

    <owl:Class rdf:about="https://kgrid.org/koio#KnowledgeObjectCollection">
        <rdfs:subClassOf rdf:resource="https://kgrid.org/koio#Collection"/>
        <obo:IAO_0000115>Knowledge Object Collection = def., two or more Knowledge Objects with a collectionIdentifer</obo:IAO_0000115>
        <rdfs:isDefinedBy rdf:resource="http://kgrid.org/koio/1.0.0/"/>
        <rdfs:label xml:lang="en">knowledge object collection</rdfs:label>
    </owl:Class>
    


    <!-- https://kgrid.org/koio#Service -->

    <owl:Class rdf:about="https://kgrid.org/koio#Service">
        <rdfs:subClassOf rdf:resource="http://purl.obolibrary.org/obo/IAO_0000030"/>
        <obo:IAO_0000115>Service, def., a Service is a defined function or capability provided by a software system. Each Service provides a way to use or interact with a KnowledgeObject, facilitating access and utilization of the Knowledge encapsulated within the KnowledgeObject.

A Service is a specification of what a self-contained piece of software does.</obo:IAO_0000115>
        <rdfs:label>service</rdfs:label>
    </owl:Class>
    


    <!-- https://kgrid.org/koio#Test -->

    <owl:Class rdf:about="https://kgrid.org/koio#Test">
        <rdfs:subClassOf rdf:resource="http://purl.obolibrary.org/obo/IAO_0000030"/>
        <obo:IAO_0000115>Test, def., an information content entity conveying a systematic procedure to assess specific aspects of software performance, functionality, or security. Tests are created to ensure that the software meets specified requirements or to identify any defects.</obo:IAO_0000115>
        <rdfs:label>test</rdfs:label>
        <rdfs:seeAlso>Test Case, Test, Test Code, Code To Be Tested
https://dev.nemo.inf.ufes.br/seon/ROoST.html

Souza ÉF, Falbo RD, Vijaykumar NL. ROoST: Reference ontology on software testing. Applied Ontology. 2017 Jan 1;12(1):59-90.</rdfs:seeAlso>
    </owl:Class>
    


    <!-- 
    ///////////////////////////////////////////////////////////////////////////////////////
    //
    // Individuals
    //
    ///////////////////////////////////////////////////////////////////////////////////////
     -->

    


    <!-- https://kgrid.org/koio#bmi.js -->

    <owl:NamedIndividual rdf:about="https://kgrid.org/koio#bmi.js">
        <rdf:type rdf:resource="http://www.ebi.ac.uk/swo/SWO_0000001"/>
    </owl:NamedIndividual>
    


    <!-- https://kgrid.org/koio#bmiAPIService -->

    <owl:NamedIndividual rdf:about="https://kgrid.org/koio#bmiAPIService">
        <rdf:type rdf:resource="http://www.ebi.ac.uk/swo/SWO_0000108"/>
        <rdf:type rdf:resource="http://www.ebi.ac.uk/swo/interface/SWO_9000054"/>
        <rdf:type rdf:resource="https://kgrid.org/koio#Service"/>
        <obo:RO_0002502 rdf:resource="https://kgrid.org/koio#bmiKnowledge"/>
        <swo:SWO_0000085 rdf:resource="https://kgrid.org/koio#index70.js"/>
        <hasDocumentation rdf:resource="https://kgrid.org/koio#bmiKOAPIDocumentation.md"/>
        <hasTest rdf:resource="https://kgrid.org/koio#bmiTestAPIService"/>
    </owl:NamedIndividual>
    


    <!-- https://kgrid.org/koio#bmiCLIService -->

    <owl:NamedIndividual rdf:about="https://kgrid.org/koio#bmiCLIService">
        <rdf:type rdf:resource="http://www.ebi.ac.uk/swo/SWO_0000108"/>
        <rdf:type rdf:resource="http://www.ebi.ac.uk/swo/interface/SWO_9000053"/>
        <rdf:type rdf:resource="https://kgrid.org/koio#Service"/>
        <obo:RO_0002502 rdf:resource="https://kgrid.org/koio#bmiKnowledge"/>
        <swo:SWO_0000085 rdf:resource="https://kgrid.org/koio#bmi_cli.ts"/>
    </owl:NamedIndividual>
    


    <!-- https://kgrid.org/koio#bmiJupiterNotebookTutorial.ipynb -->

    <owl:NamedIndividual rdf:about="https://kgrid.org/koio#bmiJupiterNotebookTutorial.ipynb">
        <rdf:type rdf:resource="https://kgrid.org/koio#InformationArtifact"/>
    </owl:NamedIndividual>
    


    <!-- https://kgrid.org/koio#bmiKO -->

    <owl:NamedIndividual rdf:about="https://kgrid.org/koio#bmiKO">
        <rdf:type rdf:resource="https://kgrid.org/koio#KnowledgeObject"/>
        <hasDocumentation rdf:resource="https://kgrid.org/koio#bmiJupiterNotebookTutorial.ipynb"/>
        <hasDocumentation rdf:resource="https://kgrid.org/koio#bmiKODocumentation.md"/>
        <hasKnowledge rdf:resource="https://kgrid.org/koio#bmiKnowledge"/>
        <hasService rdf:resource="https://kgrid.org/koio#bmiAPIService"/>
        <hasService rdf:resource="https://kgrid.org/koio#bmiCLIService"/>
        <hasTest rdf:resource="https://kgrid.org/koio#bmiTestKO.ts"/>
        <KOIOVersion rdf:datatype="http://www.w3.org/2001/XMLSchema#decimal">2.1</KOIOVersion>
    </owl:NamedIndividual>
    


    <!-- https://kgrid.org/koio#bmiKOAPIDocumentation.md -->

    <owl:NamedIndividual rdf:about="https://kgrid.org/koio#bmiKOAPIDocumentation.md">
        <rdf:type rdf:resource="https://kgrid.org/koio#InformationArtifact"/>
    </owl:NamedIndividual>
    


    <!-- https://kgrid.org/koio#bmiKODocumentation.md -->

    <owl:NamedIndividual rdf:about="https://kgrid.org/koio#bmiKODocumentation.md">
        <rdf:type rdf:resource="https://kgrid.org/koio#InformationArtifact"/>
    </owl:NamedIndividual>
    


    <!-- https://kgrid.org/koio#bmiKnowledge -->

    <owl:NamedIndividual rdf:about="https://kgrid.org/koio#bmiKnowledge">
        <rdf:type rdf:resource="https://kgrid.org/koio#Knowledge"/>
        <swo:SWO_0000085 rdf:resource="https://kgrid.org/koio#bmi.js"/>
        <hasDocumentation rdf:resource="https://kgrid.org/koio#bmiKnowledgeDocumentation.md"/>
    </owl:NamedIndividual>
    


    <!-- https://kgrid.org/koio#bmiKnowledgeDocumentation.md -->

    <owl:NamedIndividual rdf:about="https://kgrid.org/koio#bmiKnowledgeDocumentation.md">
        <rdf:type rdf:resource="https://kgrid.org/koio#InformationArtifact"/>
    </owl:NamedIndividual>
    


    <!-- https://kgrid.org/koio#bmiTestAPIService -->

    <owl:NamedIndividual rdf:about="https://kgrid.org/koio#bmiTestAPIService">
        <rdf:type rdf:resource="https://kgrid.org/koio#Test"/>
    </owl:NamedIndividual>
    


    <!-- https://kgrid.org/koio#bmiTestKO.ts -->

    <owl:NamedIndividual rdf:about="https://kgrid.org/koio#bmiTestKO.ts">
        <rdf:type rdf:resource="https://kgrid.org/koio#Test"/>
    </owl:NamedIndividual>
    


    <!-- https://kgrid.org/koio#bmiTestKnowledge.ts -->

    <owl:NamedIndividual rdf:about="https://kgrid.org/koio#bmiTestKnowledge.ts">
        <rdf:type rdf:resource="https://kgrid.org/koio#Test"/>
    </owl:NamedIndividual>
    


    <!-- https://kgrid.org/koio#bmi_cli.ts -->

    <owl:NamedIndividual rdf:about="https://kgrid.org/koio#bmi_cli.ts">
        <rdf:type rdf:resource="http://www.ebi.ac.uk/swo/SWO_0000001"/>
    </owl:NamedIndividual>
    


    <!-- https://kgrid.org/koio#index70.js -->

    <owl:NamedIndividual rdf:about="https://kgrid.org/koio#index70.js">
        <rdf:type rdf:resource="http://www.ebi.ac.uk/swo/SWO_0000001"/>
    </owl:NamedIndividual>
    


    <!-- https://kgrid.org/koio#tobacco.js -->

    <owl:NamedIndividual rdf:about="https://kgrid.org/koio#tobacco.js">
        <rdf:type rdf:resource="http://www.ebi.ac.uk/swo/SWO_0000001"/>
    </owl:NamedIndividual>
    


    <!-- https://kgrid.org/koio#tobaccoCLIService -->

    <owl:NamedIndividual rdf:about="https://kgrid.org/koio#tobaccoCLIService">
        <rdf:type rdf:resource="http://www.ebi.ac.uk/swo/SWO_0000108"/>
        <rdf:type rdf:resource="http://www.ebi.ac.uk/swo/interface/SWO_9000053"/>
        <rdf:type rdf:resource="https://kgrid.org/koio#Service"/>
        <obo:RO_0002502 rdf:resource="https://kgrid.org/koio#tobaccoKnowledge"/>
        <swo:SWO_0000085 rdf:resource="https://kgrid.org/koio#tobacco_cli.ts"/>
    </owl:NamedIndividual>
    


    <!-- https://kgrid.org/koio#tobaccoKO -->

    <owl:NamedIndividual rdf:about="https://kgrid.org/koio#tobaccoKO">
        <rdf:type rdf:resource="https://kgrid.org/koio#KnowledgeObject"/>
        <hasKnowledge rdf:resource="https://kgrid.org/koio#tobaccoKnowledge"/>
        <hasService rdf:resource="https://kgrid.org/koio#tobaccoCLIService"/>
    </owl:NamedIndividual>
    


    <!-- https://kgrid.org/koio#tobaccoKnowledge -->

    <owl:NamedIndividual rdf:about="https://kgrid.org/koio#tobaccoKnowledge">
        <rdf:type rdf:resource="https://kgrid.org/koio#Knowledge"/>
        <swo:SWO_0000085 rdf:resource="https://kgrid.org/koio#tobacco.js"/>
    </owl:NamedIndividual>
    


    <!-- https://kgrid.org/koio#tobacco_cli.ts -->

    <owl:NamedIndividual rdf:about="https://kgrid.org/koio#tobacco_cli.ts">
        <rdf:type rdf:resource="http://www.ebi.ac.uk/swo/SWO_0000001"/>
    </owl:NamedIndividual>
</rdf:RDF>



<!-- Generated by the OWL API (version 4.5.29.2024-05-13T12:11:03Z) https://github.com/owlcs/owlapi -->

